refactoring of the functional transition file in progress

theories/Environment/Stock.v
@@ -1,79 +1,80 @@
 From Coq Require Import Lia.
-From Mecha Require Import Resource Resources Term Typ REnvironment Cell SREnvironment RContext.
+From Mecha Require Import Resource Resources Term Typ REnvironment 
+                          ResourcesMap Cell SREnvironment RContext.
 From DeBrLevel Require Import LevelInterface PairLevel.
 From MMaps Require Import MMaps.
-Import ResourceNotations TermNotations CellNotations REnvironmentNotations TypNotations
+Import ResourceNotations ResourcesMapNotations 
+       TermNotations CellNotations REnvironmentNotations TypNotations
        SREnvironmentNotations ResourcesNotations SetNotations RContextNotations.
 
 (** * Environment - Virtual Resource Environment
-
-  In the functional transition there are two kind of environment: the resource environment and the stock. The former, defined in [REnvironment.v], represents the local memory during an instant. The latter, defined here, keeps local resource names with their initial value. This environment is a pair split into a map, defined in [SREnvironment.v], which maps local resource names, used for a reading interaction, to terms, and a set which keeps 'writing' local resource names.   
 *)
 
 (** ** Module - Virtual Resource Environment *)
 Module Stock <: IsLvlET.
 
-Include IsLvlPairET SREnvironment Resources.
+Include IsLvlPairET SREnvironment ResourcesMap.
+
 Module RE := REnvironment.
 Module RC := RContext.
 Module SRE := SREnvironment.
-Module RS := Resources.St.
+Module RM := ResourcesMap.
 
-Open Scope resources_scope.
-Open Scope set_scope.
+Open Scope renvironment_scope.
 
 (** *** Definitions *)
 
 (** **** Projections *)
 Definition readers (W : t) : 𝐄 := fst W.
-Definition writers (W : t) : resources := snd W.
+Definition writers (W : t) : RM.t := snd W.
 
 (** **** Empty stock 
 
   A stock is empty if and only if both components are empty.
 *)
-Definition empty : t := (∅%sr,∅). 
+Definition empty : t := (∅%sr,∅%rm). 
 
-Definition Empty (t : t) : Prop := SRE.Empty (readers t) /\ RS.Empty (writers t).
+Definition Empty (t : t) : Prop := SRE.Empty (readers t) /\ RM.Empty (writers t).
 
-Definition is_empty (t : t) : bool := SRE.Raw.is_empty (readers t) && RS.is_empty (writers t).
+Definition is_empty (t : t) : bool := SRE.Raw.is_empty (readers t) && RM.Raw.is_empty (writers t).
 
-(** **** Initialize the resource environment
-
-  For each instant, the resource environment has to be initialize for its global resource names and its local ones. The latter is done by picking information in the stock. We define [init_locals] which takes a stock [W] and a resource environment [V] and produces a new resource environment with all elements of [V] and readers and writers, stored in [W], initialized.
-*)
+(** **** Initialize the resource environment *)
 Definition init_locals (W : t) (V : 𝐕) : 𝐕 :=
-  SRE.init_readers (readers W) (RE.init_writers (writers W)  V).
+  SRE.init_readers (readers W) (RM.init_writers (writers W)  V).
 
 (** **** Update the resource environment 
 
   For each instant, the resource environment is updated at the end. Each local resources may have a new initial term for the next instant. We defined [update_locals] which takes a stock [W] and a resource environment [V] and produces a new stock.
 *)
-Definition update_locals (W : t) (V : 𝐕) : t := (SRE.update_readers (readers W) V, writers W).
+Definition update_locals_readers (W: t) (V: 𝐕) :=
+  SRE.Raw.fold (fun rr v acc => match RM.find_data rr (writers W) with
+                        | None => (⌈rr ⤆ v⌉ acc)%sr
+                        | Some rw => match V⌊rw⌋ with
+                                      | Some (⩽ … v' ⩾) =>  (⌈rr ⤆ v'⌉ acc)%sr
+                                      | _ => (⌈rr ⤆ v⌉ acc)%sr
+                                     end
+                       end) (readers W) (∅%sr).
 
-(** **** Add
+Definition update_locals (W : t) (V : 𝐕) : t := 
+  (SRE.update_readers (readers W) V, writers W).
 
-  In the stock, we add a three elements: the reader resource name [rr], the writer resource name [rw] and the initial value [v]. [rr] and [v] are added in the first member of the pair, which is a map from [ReaderStock.v], and the last elements is added in the set of writers, i.e. in the second member of the pair.
-*)
+(** **** Add *)
 Definition add (rr rw : resource) (v : Λ) (W : t) : t :=
-  (⌈ rr ⤆ v ⌉ (readers W),rw +: (writers W))%sr.
+  (⌈ rr ⤆ v ⌉ (readers W),(⌈rw ⤆ rr⌉ (writers W))%rm)%sr.
 
 (** **** Union
 
   The union between two stocks is the point-to-point union between each component.
 *)
-Definition union (W W' : t) := ((readers W ∪ readers W')%sr, writers W ∪ writers W').
+Definition union (W W' : t) := ((readers W ∪ readers W')%sr, (writers W ∪ writers W')%rm).
 
 (** **** In
 
   A resource name is in the stock if it is, at least, in one member of the stock.
 *)
-Definition In (r : resource) (W : t) := (r ∈ readers W)%sr \/ (r ∈ writers W).
+Definition In (r : resource) (W : t) := (r ∈ readers W)%sr \/ (r ∈ writers W)%rm.
 
-(** **** Find
-
-  A data can be find only in the first member of the stock.
-*)
+(** **** Find *)
 Definition find (r : resource) (W : t) := (readers W) ⌊r⌋%sr.
 
 (** **** Halts
@@ -84,7 +85,7 @@ Definition halts (k : lvl) (W : t) := SRE.halts k (readers W).
 
 (** **** New key *)
 
-Definition new_key (W : t) := max ((readers W)⁺)%sr ((writers W)⁺)%s.
+Definition new_key (W : t) := max ((readers W)⁺)%sr ((writers W)⁺)%rm.
 
 (** **** Domain equality with [RContext] *)
 
@@ -98,7 +99,7 @@ Lemma Empty_empty : Empty empty.
 Proof.
   split; simpl.
   - apply SRE.empty_1.
-  - now apply RS.empty_is_empty_2.
+  - now apply RM.empty_1.
 Qed.
 
 Lemma Empty_is_empty (t : t) : Empty t <-> is_empty t = true.
@@ -106,11 +107,11 @@ Proof.
   destruct t; unfold Empty, is_empty; simpl; split.
   - intros [HE HE'].
     apply SRE.is_empty_1 in HE; rewrite HE.
-    now apply RS.is_empty_spec.
+    now apply RM.is_empty_1 in HE'; rewrite HE'.
   - rewrite andb_true_iff. 
     intros [HE HE'].
     apply SRE.is_empty_2 in HE.
-    rewrite RS.is_empty_spec in HE'.
+    apply RM.is_empty_2 in HE'.
     now split.
 Qed. 
 
@@ -135,16 +136,17 @@ Proof.
   - intros k v HM.
     apply (HnIn k); left.
     now exists v.
-  - intros k HIn.
-    apply (HnIn k); now right.
+  - intros k v HM.
+    apply (HnIn k); right.
+    now exists v.
 Qed.
 
 Lemma Empty_notin_1 (r : resource) (t : t) : Empty t -> ~ In r t.
 Proof.
   unfold Empty, In; destruct t as [rt wt]; simpl.
-  intros [HEmp HEmp'] [[v HM] | HIn].
+  intros [HEmp HEmp'] [[v HM] | [v HM]].
   - apply (HEmp r v HM). 
-  - apply (HEmp' r HIn).
+  - apply (HEmp' r v HM).
 Qed.
 
 Lemma Empty_unfold (t: t) : Empty t -> ~(exists r, In r t).
@@ -162,10 +164,10 @@ Proof.
   split; unfold init_locals, In; destruct W as [rW wW]; simpl.
   - intro HIn. 
     apply SRE.init_readers_in_iff in HIn as [| HIn]; auto.
-    apply RE.init_writers_in_iff in HIn as [|]; auto.
+    apply RM.init_writers_in_iff in HIn as [|]; auto.
   - intro HIns. 
     apply SRE.init_readers_in_iff.
-    rewrite RE.init_writers_in_iff.
+    rewrite RM.init_writers_in_iff.
     destruct HIns as [[HIn | HIn] | HIn]; auto.
 Qed.
 
@@ -174,13 +176,13 @@ Lemma init_locals_find (r : resource) (v : 𝑣) (W : t) (V : 𝐕) :
 Proof.
   unfold init_locals, In; destruct W as [rW wW]; simpl; intro Hfi. 
   apply SRE.init_readers_find in Hfi as [| Hfi]; auto.
-  apply RE.init_writers_find in Hfi as [|]; auto.
+  apply RM.init_writers_find in Hfi as [|]; auto.
 Qed.
 
 Lemma init_locals_find_1 (r : resource) (v : 𝑣) (W : t) (V : 𝐕) :
  (init_locals W V)⌊r⌋%re = Some v -> 
  (readers W)⌊r⌋%sr = Some (Cell.extract v) \/ 
- (RE.init_writers (writers W) V)⌊r⌋%re = Some v.
+ (RM.init_writers (writers W) V)⌊r⌋%re = Some v.
 Proof.
   unfold init_locals, In; destruct W as [rW wW]; simpl; intro Hfi. 
   apply SRE.init_readers_find_1 in Hfi as [| Hfi]; auto; right.
@@ -193,7 +195,7 @@ Proof.
   unfold init_locals; intros Ht Hfi.
   apply SRE.init_readers_find_inp in Hfi; auto.
   intros r' HfV.
-  apply RE.init_writers_find_inp in HfV; auto.
+  apply RM.init_writers_find_inp in HfV; auto.
 Qed.
 
 Lemma init_locals_in_unused (W : t) (V : 𝐕) (r : resource) :
@@ -203,7 +205,7 @@ Proof.
   destruct HIn as [HIn | HIn]; simpl in *.
   - now apply SRE.init_readers_in_unused.
   - apply SRE.init_readers_unused. 
-    now apply RE.init_writers_in_unused.
+    now apply RM.init_writers_in_unused.
 Qed.
 
 Lemma init_locals_unused (r : resource) (W : t) (V : 𝐕) :
@@ -211,14 +213,14 @@ Lemma init_locals_unused (r : resource) (W : t) (V : 𝐕) :
 Proof.
   unfold Stock.init_locals; intro Hunsd.
   apply SRE.init_readers_unused.
-  now apply RE.init_writers_unused.
+  now apply RM.init_writers_unused.
 Qed.
 
 Lemma init_locals_new_key (V : 𝐕) (t : t) : ((init_locals t V)⁺)%re = max (new_key t) (V⁺)%re.
 Proof.
   destruct t; unfold init_locals, new_key; simpl.
   rewrite SRE.init_readers_new_key.
-  rewrite RE.init_writers_new_key.
+  rewrite RM.init_writers_new_key.
   lia.
 Qed.
 
@@ -278,7 +280,7 @@ Lemma empty_in (r : resource) : ~ In r empty.
 Proof.
   unfold In, empty; simpl; intros [HIn | HIn].
   - revert HIn; apply SRE.not_in_empty.
-  - inversion HIn.
+  - revert HIn; apply RM.not_in_empty.
 Qed.
 
 Lemma add_in_iff (r r' k : resource) (v : Λ) (W : t) :
@@ -288,8 +290,9 @@ Proof.
   - intros [HIn | HIn].
     -- destruct (Resource.eq_dec k r) as [| Hneq]; subst; auto. 
        rewrite SRE.add_neq_in_iff in HIn; auto.
-    -- apply RS.add_spec in HIn as [|]; auto.
-  - rewrite SRE.add_in_iff; rewrite RS.add_spec.
+    -- destruct (Resource.eq_dec k r') as [| Hneq]; subst; auto. 
+       rewrite RM.add_neq_in_iff in HIn; auto.
+  - rewrite SRE.add_in_iff; rewrite RM.add_in_iff.
     intros [Heq | [Heq | [HIn | HIn]]]; subst; auto.
 Qed.
 
@@ -297,7 +300,7 @@ Lemma union_in_iff (r : resource) (W W' : t) :
   In r (union W W') <-> In r W \/ In r W'.
 Proof.
   unfold In,union; destruct W,W'; simpl.
-  rewrite SRE.extend_in_iff; rewrite RS.union_spec.
+  rewrite SRE.extend_in_iff; rewrite RM.extend_in_iff.
   split; intros [[|] | [|]]; auto.
 Qed.
 
@@ -305,7 +308,7 @@ Lemma In_dec (r: resource) (W: t) : {In r W} + {~ In r W}.
 Proof.
   destruct W as [rW wW]; unfold In; simpl.
   destruct (SRE.In_dec rW r) as [HInrW | HnInrW];
-  destruct (RS.In_dec r wW) as [HInwW | HnInwW]; auto.
+  destruct (RM.In_dec wW r) as [HInwW | HnInwW]; auto.
   right; intros [|]; auto.
 Qed.
 
@@ -365,7 +368,7 @@ Lemma Wf_empty (k : lvl) : Wf k empty.
 Proof.
   unfold Wf, empty; simpl; split.
   - apply SRE.Wf_empty.
-  - apply Resources.Wf_empty.
+  - apply RM.Wf_empty.
 Qed.
 
 Lemma Wf_Empty (k : lvl) (t : t) : Empty t -> Wf k t.
@@ -374,8 +377,7 @@ Proof.
   - destruct H.
     now apply SRE.Wf_Empty.
   - destruct H.
-    apply RS.empty_is_empty_1 in H0; rewrite H0. 
-    apply Resources.Wf_empty.
+    now apply RM.Wf_Empty.
 Qed.
 
 Lemma Wf_add (k : lvl) (r r' : resource) (v : Λ) (W : t) :
@@ -384,8 +386,7 @@ Proof.
   unfold Wf; destruct W as [rW wW]; simpl. 
   intros Hvr Hvr' Hvv [HvrW HvwW]; split.
   - apply SRE.Wf_add; auto.
-  - apply Resources.Wf_unfold; intros r1 HIn.
-    apply RS.add_spec in HIn as [|]; subst; auto.
+  - apply RM.Wf_add; auto.
 Qed.
 
 Lemma Wf_union (k : lvl) (W W' : t) :
@@ -394,7 +395,7 @@ Proof.
   unfold Wf; destruct W,W'; simpl. 
   intros [[HvrW HvwW] [HvrW' HvwW']]; split.
   - apply SRE.Wf_extend; auto.
-  - apply Resources.Wf_union_iff; split; auto.
+  - apply RM.Wf_extend; auto.
 Qed.
 
 Lemma Wf_in (k : lvl) (r : resource) (W : t) :
@@ -403,7 +404,7 @@ Proof.
   unfold In, Wf; destruct W as [rW wW]; simpl.
   intros [HIn | HIn] [HvrW HvwW].
   - eapply SRE.Wf_in in HIn; eauto.
-  - eapply Resources.Wf_in; eauto.
+  - eapply RM.Wf_in; eauto.
 Qed.
 
 Lemma Wf_in_iff (m n k : lvl) (W : t) :
@@ -412,9 +413,9 @@ Proof.
   unfold Wf, shift, In; destruct W as [rW wW]; simpl.
   intros [Hvr Hvw]; split; intros [HIn | HIn].
   - now left; rewrite SRE.Wf_in_iff in HIn.
-  - now right; rewrite Resources.Wf_in_iff in HIn.
+  - now right; rewrite RM.Wf_in_iff in HIn.
   - now left; rewrite SRE.Wf_in_iff.
-  - now right; rewrite Resources.Wf_in_iff.
+  - now right; rewrite RM.Wf_in_iff.
 Qed.
 
 Lemma init_locals_Wf (k : lvl) (V : 𝐕) (t : t) :
@@ -424,7 +425,7 @@ Proof.
   intros [[HvrW HvrwW] HvV].
   simpl in *. unfold init_locals.
   apply SRE.init_readers_Wf; simpl; split; auto.
-  apply RE.init_writers_Wf; simpl; split; auto.
+  apply RM.init_writers_Wf; simpl; split; auto.
 Qed.
 
 (** **** [new_key] properties *)
@@ -432,10 +433,10 @@ Qed.
 Lemma new_key_empty : new_key empty = 0.
 Proof.
   unfold new_key, empty.
-  simpl (readers (∅, ∅%s) ⁺)%sr.
-  simpl (writers (∅%sr, ∅) ⁺).
+  simpl (readers (∅, ∅%rm) ⁺)%sr.
+  simpl (writers (∅%sr, ∅) ⁺)%rm.
   rewrite SRE.Ext.new_key_empty. 
-  rewrite Resources.new_key_empty.
+  rewrite RM.Ext.new_key_empty.
   now simpl. 
 Qed.
 
@@ -444,7 +445,7 @@ Proof.
   destruct t; intros []; simpl in *.
   unfold new_key; simpl.
   rewrite SRE.Ext.new_key_Empty; auto.
-  rewrite Resources.new_key_Empty; auto.
+  rewrite RM.Ext.new_key_Empty; auto.
 Qed.
 
 Lemma new_key_in (r: lvl) (t : t) : 
@@ -454,7 +455,7 @@ Proof.
   unfold In, new_key; simpl.
   intros [HIn | HIn].
   - apply SRE.Ext.new_key_in in HIn; lia.
-  - apply Resources.new_key_in in HIn; lia.
+  - apply RM.Ext.new_key_in in HIn; lia.
 Qed.
 
 Lemma new_key_union (t1 t2: t) :
@@ -462,7 +463,7 @@ Lemma new_key_union (t1 t2: t) :
 Proof.
   unfold new_key, union; destruct t1, t2; simpl.
   rewrite SRE.extend_new_key.
-  rewrite Resources.new_key_union.
+  rewrite RM.extend_new_key.
   lia.
 Qed.
 
@@ -471,7 +472,7 @@ Proof.
   unfold Wf, new_key; destruct t; simpl.
   intros [Hwf Hwf'].
   apply SRE.new_key_Wf in Hwf.
-  apply Resources.new_key_Wf in Hwf'.
+  apply RM.new_key_Wf in Hwf'.
   lia.
 Qed. 
 
@@ -479,12 +480,12 @@ Lemma new_key_add_max (m n: lvl) (v: Λ) (t: t) :
   new_key (add m n v t) = max (S m) (max (S n) (new_key t)).
 Proof.
   destruct t; unfold new_key, add. 
-  simpl (readers (⌈ m ⤆ v ⌉ readers (t0, t1), n +: writers (t0, t1)))%sr.
-  simpl (writers ((⌈ m ⤆ v ⌉ readers (t0, t1))%sr, n +: writers (t0, t1))).
+  simpl (readers (⌈ m ⤆ v ⌉ readers (t0, t1), (⌈n ⤆ m⌉  writers (t0, t1))%rm))%sr.
+  simpl (writers ((⌈ m ⤆ v ⌉ readers (t0, t1))%sr, (⌈n ⤆ m⌉  writers (t0, t1))%rm)).
   simpl (readers (t0, t1)).
   simpl (writers (t0, t1)).
   rewrite SRE.Ext.new_key_add_max.
-  rewrite Resources.new_key_add_max; lia.
+  rewrite RM.Ext.new_key_add_max; lia.
 Qed.
 
 
@@ -497,7 +498,7 @@ Proof.
   unfold new_key, shift; destruct t; simpl.
   intro Hgeq.
   rewrite SRE.shift_new_refl; try lia.
-  rewrite Resources.shift_new_refl; lia.
+  rewrite RM.shift_new_refl; lia.
 Qed.
 
 Lemma shift_in_iff (m n : lvl) (r : resource) (W : t) :
@@ -506,9 +507,9 @@ Proof.
   unfold In, shift; destruct W as [rW wW]; simpl; 
   split; intros [HIn | HIn].
   - left. now apply SRE.shift_in_iff.
-  - right; now apply Resources.shift_in_iff.
+  - right; now apply RM.shift_in_iff.
   - left. rewrite SRE.shift_in_iff; eauto.
-  - right; rewrite Resources.shift_in_iff; eauto.
+  - right; rewrite RM.shift_in_iff; eauto.
 Qed.
 
 Lemma shift_in_e (m n : lvl) (r : resource) (W : t) :
@@ -516,8 +517,7 @@ Lemma shift_in_e (m n : lvl) (r : resource) (W : t) :
 Proof.
   unfold In,shift; destruct W as [rW wW]; simpl; intros [HIn | HIn].
   - apply SRE.shift_in_e in HIn; auto.
-  - apply Resources.shift_in_e in HIn as [r' [Heq _]]; subst.
-    now exists r'.
+  - apply RM.shift_in_e in HIn; auto.
 Qed.
 
 Lemma shift_Empty_iff (m n: lvl) (W: t) :
@@ -584,7 +584,7 @@ Proof.
   unfold halts, init_locals; destruct W as [rW wW]; simpl.
   intros HvrW HvV.
   apply SRE.halts_init_readers; auto.
-  now apply RE.halts_init_writers.
+  now apply RM.halts_init_writers.
 Qed.
 
 Lemma halts_update_locals (k : lvl) (W : t) (V : 𝐕) :
@@ -726,36 +726,36 @@ Proof.
     destruct W as [rW wW]; unfold eqDom,In, new_key in *.
     simpl in HeqDom.
     simpl (readers (rW, wW)⁺)%sr.
-    simpl (writers (rW, wW)⁺).
+    simpl (writers (rW, wW)⁺)%rm.
 
     assert (HIn: (x ∈ ⌈ x ⤆ e ⌉ Rc1)%rc).
     { rewrite RC.add_in_iff; auto. }
 
     apply HeqDom in HIn as HIn'.
-    destruct HIn' as [HInr | HInw].
-    -- destruct HInr as [v HM].
-       apply SRE.find_1 in HM.
+    destruct HIn' as [[v HM] | [v' HM']].
+    -- apply SRE.find_1 in HM.
        apply SRE.add_id in HM; rewrite <- HM; clear HM.
        rewrite <- SRE.add_remove_1.
        rewrite SRE.Ext.new_key_add_max.
 
-       destruct (RS.In_dec x wW) as [HInw | HnInw].
-       + apply RS.add_remove in HInw.
-         rewrite <- HInw; clear HInw.
-         rewrite Resources.new_key_add_max.
-         rewrite (IHRc1 (SRE.Raw.remove x rW, RS.remove x wW)).
-         ++ simpl (readers (SRE.Raw.remove x rW, RS.remove x wW)).
-            simpl (writers (SRE.Raw.remove x rW, RS.remove x wW)).
+       destruct (RM.In_dec wW x) as [[v' HM'] | HnInw].
+       + apply RM.find_1 in HM'.
+         apply RM.add_id in HM'; rewrite <- HM'; clear HM'.
+         rewrite <- RM.add_remove_1.
+         rewrite RM.Ext.new_key_add_max.
+         rewrite (IHRc1 (SRE.Raw.remove x rW, RM.Raw.remove x wW)).
+         ++ simpl (readers (SRE.Raw.remove x rW, RM.Raw.remove x wW)).
+            simpl (writers (SRE.Raw.remove x rW, RM.Raw.remove x wW)).
             lia.
          ++ intro r; split; simpl.
             * intro HInRc1.
               destruct (Resource.eq_dec r x); subst; try contradiction.
               rewrite SRE.remove_in_iff.
-              rewrite RS.remove_spec.
+              rewrite RM.remove_in_iff.
               rewrite <- RC.add_neq_in_iff in HInRc1; eauto.
               apply HeqDom in HInRc1 as [|]; auto.
             * rewrite SRE.remove_in_iff.
-              rewrite RS.remove_spec.
+              rewrite RM.remove_in_iff.
               intros [[Hneq HInr] | [HInw Hneq]].
               ** rewrite <- RC.add_neq_in_iff; eauto.
                  rewrite HeqDom; auto.
@@ -778,9 +778,10 @@ Proof.
               ** destruct (Resource.eq_dec r x); subst; try contradiction.
                  rewrite <- RC.add_neq_in_iff; eauto.
                  rewrite HeqDom; auto.
-    -- apply RS.add_remove in HInw.
-       rewrite <- HInw; clear HInw.
-       rewrite Resources.new_key_add_max.
+    -- apply RM.find_1 in HM'.
+       apply RM.add_id in HM'; rewrite <- HM'; clear HM'.
+       rewrite <- RM.add_remove_1.
+       rewrite RM.Ext.new_key_add_max.
 
        destruct (SRE.In_dec rW x) as [HInr | HnInr].
 
@@ -789,35 +790,35 @@ Proof.
          apply SRE.add_id in HM; rewrite <- HM; clear HM.
          rewrite <- SRE.add_remove_1.
          rewrite SRE.Ext.new_key_add_max.
-         rewrite (IHRc1 (SRE.Raw.remove x rW, RS.remove x wW)).
-         ++ simpl (readers (SRE.Raw.remove x rW, RS.remove x wW)).
-            simpl (writers (SRE.Raw.remove x rW, RS.remove x wW)).
+         rewrite (IHRc1 (SRE.Raw.remove x rW, RM.Raw.remove x wW)).
+         ++ simpl (readers (SRE.Raw.remove x rW, RM.Raw.remove x wW)).
+            simpl (writers (SRE.Raw.remove x rW, RM.Raw.remove x wW)).
             lia.
          ++ intro r; split; simpl.
             * intro HInRc1.
               destruct (Resource.eq_dec r x); subst; try contradiction.
               rewrite SRE.remove_in_iff.
-              rewrite RS.remove_spec.
+              rewrite RM.remove_in_iff.
               rewrite <- RC.add_neq_in_iff in HInRc1; eauto.
               apply HeqDom in HInRc1 as [|]; auto.
             * rewrite SRE.remove_in_iff.
-              rewrite RS.remove_spec.
+              rewrite RM.remove_in_iff.
               intros [[Hneq HInr] | [HInw Hneq]].
               ** rewrite <- RC.add_neq_in_iff; eauto.
                  rewrite HeqDom; auto.
               ** rewrite <- RC.add_neq_in_iff; eauto.
                  rewrite HeqDom; auto.
-       + rewrite (IHRc1 (rW, RS.remove x wW)).
-         ++ simpl (readers (rW, RS.remove x wW)).
-            simpl (writers (rW, RS.remove x wW)).
+       + rewrite (IHRc1 (rW, RM.Raw.remove x wW)).
+         ++ simpl (readers (rW, RM.Raw.remove x wW)).
+            simpl (writers (rW, RM.Raw.remove x wW)).
             lia.
          ++ intro r; split; simpl.
             * intro HInRc1.
               destruct (Resource.eq_dec r x); subst; try contradiction.
-              rewrite RS.remove_spec.
+              rewrite RM.remove_in_iff.
               rewrite <- RC.add_neq_in_iff in HInRc1; eauto.
               apply HeqDom in HInRc1 as [|]; auto.
-            * rewrite RS.remove_spec.
+            * rewrite RM.remove_in_iff.
               intros [HInr | [Hneq HInw]].
               ** destruct (Resource.eq_dec r x); subst; try contradiction.
                  rewrite <- RC.add_neq_in_iff; eauto.
