theories/Environment/ResourcesMap.v
@@ -1,0 +1,411 @@
+From Coq Require Import Lia.
+From Mecha Require Import Resource Resources Resource Typ REnvironment Cell Term RContext.
+From DeBrLevel Require Import LevelInterface PairLevel MapLevelLVLD.
+From MMaps Require Import MMaps.
+Import ResourceNotations ResourceNotations CellNotations REnvironmentNotations TypNotations
+       ResourcesNotations SetNotations RContextNotations TermNotations.
+
+Module ResourcesMap <: IsLvlET.
+
+Include MakeLvlMapLVLD Resource.
+Import Raw Ext.
+
+Module RE := REnvironment.
+
+Open Scope renvironment_scope.
+
+(** *** Definition *)
+
+Definition find_data_func (c r r': resource) (v: option resource) :=
+  match v with
+    | Some _ => v
+    | None => if (Resource.eq_dec c r') then Some r else None
+  end. 
+
+Definition find_data (r: resource) (m: t) : option resource :=
+  fold (find_data_func r) m None.
+
+(** **** Initialize an environment
+*)
+Definition init_writers_func (r _: resource) (V: 𝐕) : 𝐕 := ⌈r ⤆ (⩽ unit … ⩾)⌉ V.
+
+Definition init_writers (rm: t) (V: 𝐕) := fold (init_writers_func) rm V.
+
+(** *** Properties *)
+
+(** **** [extend] properties *)
+ 
+Lemma extend_Empty_left (rm rm' : t) :
+  Empty rm -> eq (extend rm rm') rm'.
+Proof.
+  intro HEmp; unfold extend.
+  apply Empty_eq in HEmp.
+  rewrite fold_init; eauto.
+  - apply fold_identity.
+  - repeat red; intros; subst; now rewrite H1.
+Qed.
+
+Lemma extend_Empty_right (rm rm' : t) :
+  Empty rm' -> eq (extend rm rm') rm.
+Proof. intro HEmp; unfold extend; now rewrite fold_Empty; eauto. Qed.
+
+Lemma extend_add_right (r v: resource) (rm rm' : t) :
+  ~ (In r rm') -> eq (extend rm (add r v rm')) (add r v (extend rm rm')).
+Proof.
+  intro HnIn; unfold extend; rewrite fold_Add; eauto.
+  - reflexivity.
+  - intros k' k Heqk d' d Heqd c c' Heqc; subst; now rewrite Heqc.
+  - apply diamond_add.
+  - unfold Add; reflexivity.
+Qed.
+
+Lemma Wf_extend (k : lvl) (rm rm' : t) :
+  Wf k rm -> Wf k rm' -> Wf k (extend rm rm').
+Proof.
+  revert rm; induction rm' using map_induction; intros rm Hvrs Hvrs'.
+  - rewrite extend_Empty_right; auto.
+  - unfold Add in H0; rewrite H0 in *; clear H0.
+    rewrite extend_add_right; auto.
+    apply Wf_add_notin in Hvrs' as [Hvx [Hve Hvrs'1]]; auto.
+    apply Wf_add; auto.
+Qed.
+
+Lemma extend_new_key (rm rm': t) :
+  new_key (extend rm rm') = max (new_key rm) (new_key rm').
+Proof.
+  revert rm.
+  induction rm' using map_induction; intro rm.
+  - rewrite extend_Empty_right; auto.
+    rewrite (new_key_Empty rm'); auto; lia.
+  - unfold Add in H0; rewrite H0; clear H0.
+    rewrite extend_add_right; auto.
+    do 2 rewrite new_key_add_max.
+    rewrite IHrm'1; lia.
+Qed.
+
+(** **** [new_key] properties *)
+
+Lemma new_key_Wf (k: lvl) (rm: t) : Wf k rm -> new_key rm <= k.
+Proof.
+  induction rm using map_induction; intro Hwf.
+  - rewrite new_key_Empty; auto; lia.
+  - unfold Add in H0; rewrite H0 in *; clear H0.
+    apply Wf_add_notin in Hwf as [Hwfx [_ Hwf]]; auto.
+    apply IHrm1 in Hwf.
+    unfold Resource.Wf in Hwfx.
+    rewrite new_key_add_max; lia.
+Qed.
+
+(** **** [init_writers] properties *)
+
+#[export] Instance init_writers_func_eq : 
+  Proper (Logic.eq ==> Logic.eq ==> RE.eq ==> RE.eq) init_writers_func.
+Proof. 
+  unfold init_writers_func; intros k' k Heqk v' v Heqv V V' HeqV. 
+  subst; now rewrite HeqV. 
+Qed.
+
+Lemma init_writers_diamond : Diamond RE.eq init_writers_func.
+Proof.
+  intros k k' v v' rm rm' rm1' Hneq Heq Heq'.
+  unfold init_writers_func in *.
+  rewrite <- Heq, <- Heq'.
+  rewrite RE.add_add_2; auto; reflexivity.
+Qed.
+
+#[export] Instance renvironment_equiv_eq : Equivalence RE.eq := RE.eq_equiv.
+
+#[local] Hint Resolve init_writers_func_eq renvironment_equiv_eq 
+                      init_writers_diamond : core.
+
+Lemma init_writers_Empty (rm: t) (V: 𝐕) : Empty rm -> ((init_writers rm V) = V)%re.
+Proof.
+  intro Hemp; unfold init_writers.
+  rewrite fold_Empty; now auto.
+Qed.
+
+Lemma init_writers_add (r v: resource) (rm: t) (V: 𝐕) :
+  ~(In r rm) ->
+  ((init_writers (add r v rm) V) = (⌈r ⤆ (⩽ unit … ⩾)⌉ (init_writers rm V)))%re. 
+Proof.
+  unfold init_writers; intro HnIn.
+  rewrite fold_add; auto.
+  now unfold init_writers_func at 1.
+Qed.
+
+#[export] Instance init_writers_eq : Proper (eq ==> RE.eq ==> RE.eq) init_writers.
+Proof.
+  intros rm rm' Heqrm V V' HeqV; unfold init_writers.
+  rewrite fold_init; eauto.
+  clear V HeqV; revert rm' Heqrm.
+  induction rm using map_induction; intros rm' Heq.
+  - do 2 (rewrite init_writers_Empty; auto).
+    -- reflexivity.
+    -- now rewrite <- Heq.
+  - rewrite fold_Add; eauto.
+    rewrite fold_Add with (m1 := rm1) (m2 := rm'); eauto.
+    -- reflexivity.
+    -- now unfold Add in *; rewrite <- Heq.
+Qed.
+
+Lemma init_writers_in_unused (rm: t) (V: 𝐕) (r: resource) :
+  (In r rm) -> RE.unused r (init_writers rm V).
+Proof.
+  revert r; induction rm using map_induction; intro r.
+  - intros [v HM].
+    exfalso; apply (H r v HM).
+  - intro HIn. 
+    unfold Add in H0; rewrite H0 in *; clear H0. 
+    rewrite init_writers_add; auto.
+    apply add_in_iff in HIn as [| HIn]; subst. 
+    -- apply RE.unused_add_eq; now red.
+    -- assert (r <> x) by (intro; subst; contradiction).
+       apply RE.unused_add_neq; auto. 
+Qed.
+
+Lemma init_writers_find (rm: t) (V: 𝐕) (r: resource) (v: 𝑣) :
+  (init_writers rm V)⌊r⌋ = Some v -> (In r rm) \/ V⌊r⌋ = Some v.
+Proof.
+  revert r v; induction rm using map_induction; intros r v Hfi.
+  - rewrite init_writers_Empty in Hfi; auto.
+  - unfold Add in H0; rewrite H0 in *; clear H0.
+    rewrite init_writers_add in Hfi; auto.
+    destruct (Resource.eq_dec x r) as [Heq | Hneq]; subst.
+    -- left; rewrite add_in_iff; auto.
+    -- rewrite RE.add_neq_o in Hfi; auto.
+       apply IHrm1 in Hfi as [HIn | Hfi]; auto.
+       left; rewrite add_in_iff; auto.
+Qed.
+
+Lemma init_writers_find_inp (rm: t) (V: 𝐕) (r: resource) (v: 𝑣) :
+  (forall r, V⌊r⌋ = Some v -> exists v', Logic.eq v (Cell.inp v')) ->
+  (init_writers rm V)⌊r⌋ = Some v -> exists v', Logic.eq v (Cell.inp v'). 
+Proof.
+  revert r v; induction rm using map_induction; intros r v Ht Hfi.
+  - rewrite init_writers_Empty in Hfi; auto.
+    now apply (Ht r).
+  - unfold Add in H0; rewrite H0 in *; clear H0.
+    rewrite init_writers_add in Hfi; auto.
+    destruct (Resource.eq_dec x r) as [Heq | Hneq]; subst.
+    -- rewrite RE.add_eq_o in Hfi; auto.
+       inversion Hfi; subst; now exists Term.tm_unit.
+    -- rewrite RE.add_neq_o in Hfi; auto.
+       now apply (IHrm1 r).
+Qed.
+
+Lemma init_writers_in_iff (rm: t) (V: 𝐕) (r: resource) :
+  r ∈ (init_writers rm V) <-> (In r rm) \/ r ∈ V.
+Proof.
+  revert r; induction rm using map_induction; intro r; split.
+  - intro HIn. rewrite init_writers_Empty in HIn; auto.
+  - intros [[v HM] | HIn].
+    -- exfalso.
+       now apply (H r v).
+    -- now rewrite init_writers_Empty.
+  - intro HIn; unfold Add in H0; rewrite H0 in *; clear H0. 
+    rewrite init_writers_add in HIn; auto.
+    apply RE.add_in_iff in HIn as [Heq | HIn]; subst.
+    -- left; rewrite add_in_iff; auto.
+    -- apply IHrm1 in HIn as [HIn | HIn]; auto.
+       left; rewrite add_in_iff; auto.
+  - intros [HIn | HIn]; unfold Add in H0; rewrite H0 in *; clear H0.
+    -- rewrite init_writers_add; auto.
+       rewrite RE.add_in_iff.
+       apply add_in_iff in HIn as [Heq | HIn]; auto.
+       right; rewrite IHrm1; now left.
+    -- rewrite init_writers_add; auto.
+       rewrite RE.add_in_iff; right.
+       rewrite IHrm1; now right. 
+Qed. 
+
+Lemma init_writers_in (rm: t) (V: 𝐕) (r: resource) :
+  (In r rm) -> (init_writers rm V)⌊r⌋ = Some (Cell.inp <[unit]>).
+Proof.
+  revert r; induction rm using map_induction; intros r HIn.
+  - destruct HIn as [v HM]. 
+    exfalso; now apply (H r v).
+  - unfold Add in H0; rewrite H0 in *; clear H0.
+    rewrite init_writers_add; auto.
+    destruct (Resource.eq_dec r x) as [| Hneq]; subst.
+    -- now rewrite RE.add_eq_o.
+    -- rewrite RE.add_neq_o; auto.
+       apply add_in_iff in HIn as [| HIn]; subst; auto.
+       contradiction.
+Qed.
+
+Lemma init_writers_unused (r: resource) (rm: t) (V: 𝐕) :
+  RE.unused r V -> RE.unused r (init_writers rm V).
+Proof.
+  revert r; induction rm using map_induction; intro r.
+  - rewrite init_writers_Empty; auto.
+  - unfold Add in H0; rewrite H0 in *; clear H0.
+    rewrite init_writers_add; auto.
+    destruct (Resource.eq_dec r x) as [| Hneq]; subst; intro Hunsd.
+    -- apply RE.unused_add_eq; now red.
+    -- apply RE.unused_add_neq; auto.
+Qed.
+
+Lemma init_writers_add_remove (r v: resource) (rm: t) (V: 𝐕) :
+  ((init_writers (add r v rm) V) = (init_writers (add r v rm) (RE.Raw.remove r V)))%re.
+Proof.
+  revert r V; induction rm using map_induction; intros r V.
+  - assert (HnIn: ~ In r rm).
+    { intros [v' HM]; now apply (H r v'). } 
+    do 2 (rewrite init_writers_add; auto).
+    do 2 (rewrite init_writers_Empty; auto).
+    induction V using RE.map_induction.
+    -- assert (HnIn': r ∉ V).
+       { intros [v' HM]; now apply (H0 r v'). } 
+       rewrite <- RE.remove_id in HnIn'.
+       now rewrite HnIn'.
+    -- unfold RE.Add in H1; rewrite H1 in *; clear H1.
+       destruct (Resource.eq_dec r x) as [| Hneq]; subst.
+        + rewrite RE.add_shadow.
+          rewrite RE.add_remove_1.
+          now rewrite RE.add_shadow.
+        + rewrite RE.add_add_2; auto.
+          rewrite RE.remove_add_2; auto.
+          symmetry.
+          rewrite RE.add_add_2; auto.
+          now rewrite IHV1.
+  - unfold Add in H0; rewrite H0 in *; clear H0. 
+    destruct (Resource.eq_dec r x) as [| Hneq]; subst.
+    -- rewrite add_shadow.
+       now rewrite IHrm1.
+    -- rewrite add_add_2; auto.
+       do 2 rewrite (init_writers_add x) 
+       by (rewrite add_in_iff; intros [|]; auto).
+       now rewrite <- IHrm1.
+Qed.
+
+Lemma init_writers_new_key (V: 𝐕) (rm: t) : 
+  (init_writers rm V)⁺ = max (new_key rm) (V⁺).
+Proof.
+  revert V.
+  induction rm using map_induction; intro V.
+  - rewrite new_key_Empty; auto; simpl.
+    rewrite init_writers_Empty; auto.
+  - unfold Add in H0; rewrite H0 in *; clear H0.
+    rewrite init_writers_add_remove.
+    rewrite init_writers_add; auto.
+    rewrite new_key_add_max; auto.
+    rewrite RE.Ext.new_key_add_max.
+    rewrite IHrm1.
+    destruct (RE.In_dec V x).
+    + apply RE.new_key_in_remove_1 in i as HI.
+      rewrite HI; lia.
+    + apply RE.remove_id in n.
+      rewrite n; lia.
+Qed.
+
+Lemma init_writers_Wf (k : lvl) (V: 𝐕) (t : t) :
+  (Wf k t) /\ k ⊩ V -> k ⊩ (init_writers t V).
+Proof.
+  revert k V.
+  induction t using map_induction; intros k V  [Hvt HvV].
+  - rewrite init_writers_Empty; auto.
+  - unfold Add in H0; rewrite H0 in *; clear H0.
+    apply Wf_add_notin in Hvt as [Hvx [Hve Hvt1]]; auto.
+    rewrite init_writers_add_remove.
+    rewrite init_writers_add; auto.
+    apply RE.Wf_add_notin.
+    -- rewrite init_writers_in_iff; intros [|]; auto.
+       apply RE.remove_in_iff in H0 as []; auto.
+    -- do 2 (split;auto).
+       + constructor.
+       + apply IHt1; split; auto.
+         now apply RE.Wf_remove.
+Qed.
+
+(** **** [halts] properties *)
+
+Lemma halts_init_writers (k : lvl) (rm: t) (V: 𝐕) :
+  RE.halts k V -> RE.halts k (init_writers rm V).
+Proof.
+  induction rm using map_induction; intro Hlt.
+  - now rewrite init_writers_Empty.
+  - unfold Add in *; rewrite H0 in *; clear H0.
+    rewrite init_writers_add; auto.
+    apply RE.halts_add; split; auto.
+    red; exists <[unit]>; split.
+    -- apply Evaluation_Transition.multi_unit.
+    -- now constructor.
+Qed.
+
+(** *** Morphisms *)
+
+#[export] Instance resourcesmap_in_iff : Proper (Logic.eq ==> eq ==> iff) In.
+Proof. intros k' k Heqk rm rm' Heqrs; subst; now rewrite Heqrs. Qed.
+
+#[export] Instance resourcesmap_Add_iff : 
+  Proper (Resource.eq ==> Resource.eq ==> eq ==> eq ==> iff) (@Add Resource.t).
+Proof.
+  intros k' k Heqk d d' Heqd rm rm' Heqrs rs1 rs1' Heqrs1; unfold Add.
+  now rewrite Heqk, Heqd, Heqrs, Heqrs1. 
+Qed.
+
+End ResourcesMap.
+
+(** ---- *)
+
+(** ** Notation - Virtual Resource Environment - Reader *)
+
+Module ResourcesMapNotations.
+
+(** *** Scope *)
+Declare Scope rmap_scope.
+Delimit Scope rmap_scope with rm.
+
+(** *** Notations *)
+
+Notation "t '⁺'" := (ResourcesMap.Ext.new_key t) (at level 16) : rmap_scope.
+Notation "∅" := ResourcesMap.Raw.empty (at level 0, no associativity) : rmap_scope. 
+Notation "r '∉' t" := (~ (ResourcesMap.Raw.In r t)) (at level 75, no associativity) : rmap_scope. 
+Notation "'isEmpty(' t ')'" := (ResourcesMap.Empty t) (at level 20, no associativity) : rmap_scope. 
+Notation "t '⌊' x '⌋'"  := (ResourcesMap.Raw.find x t) (at level 15, x constr) : rmap_scope.
+Notation "'max(' t ')'"  := (ResourcesMap.Ext.max_key t) (at level 15) : rmap_scope.
+Notation "⌈ x ⤆ v '⌉' t" := (ResourcesMap.Raw.add x v t) 
+                             (at level 15, x constr, v constr) : rmap_scope.
+Notation "'[⧐' lb '–' k ']' t" := (ResourcesMap.shift lb k t) 
+                                   (at level 65, right associativity) : rmap_scope.
+
+Infix "⊆" := ResourcesMap.Submap (at level 60, no associativity) : rmap_scope. 
+Infix "∈" := ResourcesMap.Raw.In (at level 60, no associativity) : rmap_scope. 
+Infix "=" := ResourcesMap.eq : rmap_scope.
+Infix "∪" := ResourcesMap.extend : rmap_scope.
+Infix "⊩" := ResourcesMap.Wf (at level 20, no associativity) : rmap_scope.
+
+(** *** Morphisms *)
+
+Import ResourcesMap.
+
+#[export] Instance resourcesmap_equiv_eq : Equivalence ResourcesMap.eq := _.
+
+#[export] Instance resourcesmap_max_eq : Proper (eq ==> Logic.eq) (Ext.max_key) := Ext.max_key_eq.
+
+#[export] Instance resourcesmap_new_eq : Proper (eq ==> Logic.eq) (Ext.new_key) := Ext.new_key_eq.
+
+#[export] Instance resourcesmap_in_iff : 
+  Proper (Logic.eq ==> ResourcesMap.eq ==> iff) (ResourcesMap.Raw.In) := _.
+
+#[export] Instance resourcesmap_find_eq : Proper (Logic.eq ==> eq ==> Logic.eq) (Raw.find) := _.
+
+#[export] Instance resourcesmap_Empty_iff : 
+  Proper (ResourcesMap.eq ==> iff) (ResourcesMap.Empty) := _.
+
+#[export] Instance resourcesmap_Add_iff : 
+  Proper (Resource.eq ==> Resource.eq ==> eq ==> eq ==> iff) (@ResourcesMap.Add Resource.t) := _.
+
+#[export] Instance resourcesmap_add_eq : 
+  Proper (Resource.eq ==> Resource.eq ==> eq ==> eq) (@Raw.add Resource.t) := _.
+
+#[export] Instance resourcesmap_Submap_iff : Proper (eq ==> eq ==> iff) Submap := _.
+
+#[export] Instance resourcesmap_Submap_po : PreOrder ResourcesMap.Submap := Submap_po.
+
+#[export] Instance resourcesmap_Wf_iff : 
+  Proper (Logic.eq ==> ResourcesMap.eq ==> iff) ResourcesMap.Wf := _.
+
+#[export] Instance resourcesmap_shift_eq : Proper (Logic.eq ==> Logic.eq ==> eq ==> eq) shift := _.
+
+End ResourcesMapNotations.
